\documentclass[12pt, paper=letter]{scrartcl}

\usepackage{../../utils/jtinoco.eng.v1}

\title {\Large EXCL Season 4 Assignment 5}
\date{12 June 2025}
\author{Jordan Tinoco}

\begin{document}
    \maketitle

    \begin{problem*}
        Positive $a,b,c$ satisfy $a + b + c = 1$.
        Prove that
        \[
            \frac{ab + c}{a + b} + \frac{bc + a}{b + c} + \frac{ca + b}{c + a} \geq 2.
        \]
    \end{problem*}
    \begin{solution*}
        By $a + b + c = 1$ we have $c = 1 - a - b$, thus $ab + c = ab - a - b + 1 = (1 - a)(1 - b)$, and $a + b = 1 - c$.
        Likewise for $(bc + a)$ and $(ca + b)$, we found that original inequality is equivalent to
        \[
            \frac{(1 - a)(1 - b)}{(1 - c)} + \frac{(1 - b)(1 - c)}{(1 - a)} + \frac{(1 - c)(1 - a)}{(1 - b)} \geq 2.
        \]
        Let $x = 1 - a$, $y = 1 - b$ and $z = 1 - c$, with $x + y + z = 3 - (a + b + c) = 2$, we have
        \[
            \frac{xy}{z} + \frac{yz}{x} + \frac{zx}{y} \geq 2.
        \]
        By Cauchy-Schwarz,
        \begin{align*}
            \left(\frac{zx}{y} + \frac{xy}{z} + \frac{yz}{x}\right)\left(\frac{xy}{z} + \frac{yz}{x} + \frac{zx}{y}\right) &\geq (x + y + z)^2\\[3mm]
            \iff \frac{xy}{z} + \frac{yz}{x} + \frac{zx}{y} &\geq x + y + z\\[2mm]
            \implies \frac{xy}{z} + \frac{yz}{x} + \frac{zx}{y} &\geq 2.
        \end{align*}
    \end{solution*}

    \begin{problem*}
        If $a,b,c > 0$, prove that
        \[
            \frac{3(ab + bc + ca)}{2(a + b + c)} \geq \frac{ab}{a + b} + \frac{bc}{b + c} + \frac{ca}{c + a}.
        \]
    \end{problem*}
    \begin{solution*}
        Multiplying by $a + b + c$, we have
        \begin{align*}
            \iff \frac{3(ab + bc + ca)}{2} &\geq (a + b + c)\left(\frac{ab}{a + b} + \frac{bc}{b + c} + \frac{ca}{c + a}\right)\\[3mm]
            \iff \frac{3(ab + bc + ca)}{2} &\geq \left(\frac{abc}{a + b} + \frac{abc}{b + c} + \frac{abc}{c + a}\right) + (ab + bc + ca)\\[3mm]
            \iff \frac{ab + bc + ca}{2} &\geq abc\left(\frac{1}{a + b} + \frac{1}{b + c} + \frac{1}{c + a}\right)\\[3mm]
            \iff \frac{1}{a} + \frac{1}{b} + \frac{1}{c} &\geq 2\left(\frac{1}{a + b} + \frac{1}{b + c} + \frac{1}{c + a}\right)
        \end{align*}
        By AM-HM inequality, we know that $\frac{1}{a} + \frac{1}{b} \geq \frac{4}{a + b}$, $\frac{1}{b} + \frac{1}{c} \geq \frac{4}{b + c}$ and $\frac{1}{c} + \frac{1}{a} \geq \frac{4}{c + a}$ adding these inequalities we obtain the result.
    \end{solution*}
    
    \begin{problem*}
        If $a,b,c > 0$, prove that
        \[
            \frac{a}{(b + c)^2} + \frac{b}{(c + a)^2} + \frac{c}{(a + b)^2} \geq \frac{9}{4(a + b + c)}
        \]
    \end{problem*}
    \begin{solution*}
        Since the inequality is homogeneous, we may assume WLOG that $a + b + c = 3$.
        So the inequality we wish to prove is
        \[
            \frac{a}{(3 - a)^2} + \frac{b}{(3 - b)^2} + \frac{c}{(3 - c)^2} \geq \frac{3}{4}.
        \]
        Consider the function $f(x) = \frac{x}{(3 - x)^2}$ for $x \neq 3$, the second derivate of this function is $f''(x) = \frac{2x + 12}{(3 - x)^4}$, which is convex for $x > 0$.
        Using Jensen's inequality, we have
        \begin{align*}
            \frac{f(a) + f(b) + f(c)}{3} &\geq f \left(\frac{a + b + c }{3}\right)\\[3mm]
            \iff f(a) + f(b) + f(c) &\geq 3 f(1)\\[3mm]
            \iff f(a) + f(b) + f(c) &\geq 3 \left(\frac{1}{(3 - 1)^2}\right) = \frac{3}{4}
        \end{align*}
    \end{solution*}

    \begin{problem*}
        If $a,b,c > 0$ are the sides of a triangle, find the minimum value of
        \[
            \frac{\sqrt {a}}{\sqrt {b} + \sqrt {c} - \sqrt {a}} + \frac{\sqrt {b}}{\sqrt {c} + \sqrt {a} - \sqrt {b}} + \frac{\sqrt {c}}{\sqrt {a} + \sqrt {b} - \sqrt {c}}.
        \]
    \end{problem*}
    \begin{solution*}
        Let $x = \sqrt {b} + \sqrt {c} - \sqrt {a}$, $\quad y = \sqrt {c} + \sqrt {a} - \sqrt {b}\quad$ and $\quad z = \sqrt {a} + \sqrt {b} - \sqrt {c}$.

        We have that $y + z = 2 \sqrt {a} \iff \sqrt {a} = \frac{y + z}{2}$, likewise, for $\sqrt {b}$ and $\sqrt {c}$.
        Thus, the expression is equal to
        \begin{align*}
            \frac{x + y}{2z} + \frac{y + z}{2x} + \frac{z + x}{2y}
            \iff \frac{1}{2} \left(\frac{x}{y} + \frac{y}{x} + \frac{y}{z} + \frac{z}{y} + \frac{z}{x} + \frac{x}{z}\right)
            \geq \frac{1}{2} (2 + 2 + 2) = 3.
        \end{align*}
    \end{solution*}
\end{document}